

106 (5分)

$$2. \quad x^{\frac{2}{3}} + y^{\frac{2}{3}} = 5 \Rightarrow \frac{2}{3}x^{-\frac{1}{3}} + \frac{2}{3}y^{-\frac{1}{3}} \frac{dy}{dx} = 0 \Rightarrow \frac{dy}{dx} = -\frac{y}{x} \Rightarrow m = -\frac{1}{2} \Rightarrow y-1 = -\frac{1}{2}(x-8) \Rightarrow y = -\frac{1}{2}x + 5$$

$$3. (a) \quad \frac{dy}{dx} = \frac{1}{2}(e^x + e^{-x})^{\frac{1}{2}}(2e^x - 2e^{-x}) = \frac{e^x - e^{-x}}{\sqrt{e^x + e^{-x}}}$$

$$(b) \quad y = \frac{1}{4}\ln(x+1) - \frac{1}{4}\ln(x-1) + \frac{1}{2}\tan^{-1}x \Rightarrow \frac{dy}{dx} = \frac{1}{4(x+1)} - \frac{1}{4(x-1)} + \frac{1}{2(x^2+1)}$$

$$(c) \quad \frac{dy}{dx} = 2x \log_2(x^2+1) + x^2 \frac{1}{\ln 2} \cdot \frac{2x}{x^2+1}$$

$$(d) \quad x = \sec \frac{1}{y} \Rightarrow \sec^2 x = \frac{1}{y} \Rightarrow -y^{-2} \frac{dy}{dx} = \frac{1}{x\sqrt{x^2-1}} \Rightarrow \frac{dy}{dx} = \frac{-y^2}{x\sqrt{x^2-1}} = \frac{-1}{(\sec x)\sqrt{\sec^2 x - 1}} \\ (y = \frac{1}{\sec x})$$

105 (5分)

$$2. \quad y = \frac{x+1}{x-1} = 1 + \frac{2}{x-1} \quad \frac{dy}{dx} = -2(x-1)^{-2} = -\frac{1}{2} \Rightarrow x=3 \text{ 或 } -1 \quad \text{切点为 } (3, 2) \text{ 或 } (-1, 0)$$

$$\text{所求 } y+x=1 \text{ 或 } y+x=-1$$

$$3. (a) \quad y = e^{(\ln|5x| + (\cos x)^2)} \Rightarrow \frac{dy}{dx} = e^{(\ln|5x| + (\cos x)^2)} \cdot 2(\ln|5x| + (\cos x)^2) \left(\frac{1}{x} - 2\cos x \sin x \right) \\ \text{或 } -\sin 2x \quad \uparrow$$

$$(b) \quad y = \tan^{-1}(\sqrt{1-x^2}) \Rightarrow \frac{dy}{dx} = \frac{1}{(\sqrt{1-x^2})^2 + 1} \cdot \frac{1}{2}(1-x^2)^{-\frac{1}{2}} \cdot (-2x) = \frac{-x}{2-x^2} \cdot \frac{1}{\sqrt{1-x^2}}$$

$$4. \quad x^2 + \sqrt{xy} + y^2 = 72, (x_0, y_0) = (2, 8) \Rightarrow 2x + \frac{1}{2}x^{-\frac{1}{2}}y^{\frac{1}{2}} + x^{\frac{1}{2}}\frac{1}{2}y^{-\frac{1}{2}}\frac{dy}{dx} + 2y\frac{dy}{dx} = 0$$

$$\Rightarrow \frac{dy}{dx} = \frac{-(2x + \frac{1}{2}x^{-\frac{1}{2}}y^{\frac{1}{2}})}{2y + \frac{1}{2}x^{\frac{1}{2}}y^{-\frac{1}{2}}}$$

$$\text{故过 } (2, 8) \text{ 的切线斜率} = \frac{-(4 + \frac{1}{2}\frac{\sqrt{8}}{2})}{16 + \frac{1}{2}\frac{\sqrt{8}}{2}} = \frac{-(5)}{16 + \frac{1}{4}} = \frac{-4}{13}$$

$$\text{所求: } y-8 = \frac{-4}{13}(x-2)$$

$$5. \quad f(x) = x^3 + x - 1 \\ f'(x) = 3x^2 + 2$$

$$(f^{-1}(x))' = \frac{1}{f'(f^{-1}(x))} \Rightarrow (f^{-1}(-4))' = \frac{1}{f'(f^{-1}(-4))} = \frac{1}{f'(-1)} = \frac{1}{5}$$

$$\left(\begin{aligned} x^3 + x - 1 &= -4 \Rightarrow x^3 + x + 3 = 0 \Rightarrow (x+1)(x^2 - x + 3) = 0 \\ &\Rightarrow x = -1 \end{aligned} \right)$$

104 (分部)

$$3. (a) y = 2^x \left(1 - \frac{4}{x+3}\right) \Rightarrow \frac{dy}{dx} = \ln 2 \cdot 2^x \left(1 - \frac{4}{x+3}\right) + 2^x \left(4(x+3)^{-2}\right) = \ln 2 \cdot 2^x \left(1 - \frac{4}{x+3}\right) + \frac{2^{x+2}}{(x+3)^2}$$

$$(b) y = \left(\ln \frac{3}{x}\right)^{\frac{x}{3}} = e^{\frac{x}{3} \ln(\ln \frac{3}{x})}$$

$$\begin{aligned} \frac{dy}{dx} &= \left(\ln \frac{3}{x}\right)^{\frac{x}{3}} \cdot \left(\frac{\ln(\ln \frac{3}{x})}{3} + \frac{1}{3} \cdot \frac{1}{\ln \frac{3}{x}} \cdot \left(-\frac{1}{x}\right)\right) = \left(\ln \frac{3}{x}\right)^{\frac{x}{3}} \cdot \frac{\ln(\ln \frac{3}{x}) - \ln \frac{x}{3}}{3} \\ &= \frac{\ln(\ln \frac{3}{x}) \cdot \ln(\frac{3}{x})^{\frac{x}{3}} - (\ln \frac{3}{x})^{\frac{x+3}{3}}}{3} \end{aligned}$$

$$\begin{aligned} (c) y &= e^{3x} \sin(\cos^2(3x)) = 3e^{3x} \sin(\cos^2(3x)) + e^{3x} \cos(\cos^2(3x)) \cdot 2\cos 3x \cdot -\sin 3x \cdot 3 \\ &= 3e^{3x} \sin(\cos^2(3x)) - 3e^{3x} \cos(\cos^2(3x)) \sin 6x \end{aligned}$$

$$(d) y = \sqrt{2 + \sqrt{2 + \sqrt{x}}} = \frac{1}{2} \cdot \frac{1}{\sqrt{2 + \sqrt{2 + \sqrt{x}}}} \cdot \frac{1}{2} \cdot \frac{1}{\sqrt{2 + \sqrt{x}}} \cdot \frac{1}{2} \cdot \frac{1}{\sqrt{x}} = \frac{1}{8 \cdot \sqrt{2 + \sqrt{2 + \sqrt{x}}} \cdot \sqrt{2 + \sqrt{x}} \cdot \sqrt{x}}$$

$$\begin{aligned} (e) \ln(xy) - e^{x+y} + x^2y &= 1 \Rightarrow \frac{1}{x} + \frac{1}{y} \frac{dy}{dx} - e^x e^y - e^x e^y \frac{dy}{dx} + xy + x^2 \frac{dy}{dx} = 0 \\ \Rightarrow \frac{dy}{dx} &= \frac{-\frac{1}{x} + e^{x+y} - xy}{x^2 - e^{x+y} + \frac{1}{y}} = \frac{-y + xy e^{x+y} - x^2 y^2}{x^2 y + x - xy e^{x+y}} \end{aligned}$$

103 (分部)

$$\begin{aligned} 2. (a) y &= \left(\frac{\cos x}{1 + \sin x}\right)^2 \Rightarrow \frac{dy}{dx} = 2 \cdot \frac{\cos x}{1 + \sin x} \cdot \frac{(-\sin x)(1 + \sin x) - \cos x \cdot \cos x}{(1 + \sin x)^2} = 2 \cdot \frac{\cos x}{1 + \sin x} \cdot \frac{-\sin x - 1}{(1 + \sin x)^2} \\ &= \frac{-2 \cos x}{(1 + \sin x)^2} \end{aligned}$$

$$\begin{aligned} (b) x \cdot \sin 5y &= y \cos 5x + \frac{1}{2} \Rightarrow \sin 5y + x \cos 5y \cdot 5 \frac{dy}{dx} = \frac{dy}{dx} \cos 5x - 5y \sin 5x \\ \Rightarrow \frac{dy}{dx} &= \frac{-5y \sin 5x - \sin 5y}{5x \cos 5y - \cos 5x} \end{aligned}$$

$$(c) y = \ln(1 + \tan^{-1} x^3) \Rightarrow \frac{dy}{dx} = \frac{1}{\tan^{-1} x^3} \cdot \frac{3x^2}{1 + x^6}$$

$$\begin{aligned} (d) y &= \int \frac{x^5(x+1)^6}{(x+2)} \Rightarrow \ln y = \frac{5}{3} \ln x + \frac{16}{3} \ln(x+1) - \frac{1}{3} \ln(x+2) \\ \Rightarrow \frac{1}{y} \frac{dy}{dx} &= \frac{5}{3} \cdot \frac{1}{x} + \frac{16}{3} \cdot \frac{1}{x+1} - \frac{1}{3} \cdot \frac{1}{x+2} \\ \Rightarrow \frac{dy}{dx} &= \int \frac{x^5(x+1)^6}{x+2} \left(\frac{5}{3} \cdot \frac{1}{x} + \frac{16}{3} \cdot \frac{1}{x+1} - \frac{1}{3} \cdot \frac{1}{x+2} \right) \end{aligned}$$

102 (5/23)

$$2. (a) y = \frac{\sin x - x}{x^3} \Rightarrow \frac{dy}{dx} = \frac{(\cos x - 1)x^3 - (\sin x - x)3x^2}{x^6} = \frac{2x + x \cos x - 3 \sin x}{x^4}$$

$$(b) y = e^{2x} \cdot x^5 \cdot \sin x \Rightarrow \frac{dy}{dx} = 2e^{2x} \cdot x^5 \sin x + 5x^4 \cdot e^{2x} \sin x + e^{2x} x^5 \cos x$$

$$(c) y = \cos x^{\sqrt{3}} \Rightarrow \frac{dy}{dx} = -\sin x^{\sqrt{3}} \cdot \sqrt{3} \cdot x^{\sqrt{3}-1}$$

$$(d) y = (\cos x)^{\sqrt{3}} \Rightarrow y = e^{\sqrt{3} \ln \cos x} \Rightarrow \frac{dy}{dx} = (\cos x)^{\sqrt{3}} \cdot \sqrt{3} \cdot \frac{-\sin x}{\cos x} \\ = -\sqrt{3} \sin x \cdot (\cos x)^{\sqrt{3}-1} \\ \Rightarrow -\sqrt{3} (\cos x)^{\sqrt{3}} \cdot \tan x$$

$$(e) y = \sqrt{3}^{\sin x} + \sqrt{3} \tan x + \sec(\sqrt{3}x) \Rightarrow \frac{dy}{dx} = \sqrt{3}^{\sin x} \cdot (\ln \sqrt{3} \cdot \cos x) + \sqrt{3} \sec^2 x + \sec(\sqrt{3}x) \tan(\sqrt{3}x) \sqrt{3} \\ = e^{\sin x \ln \sqrt{3}} + \sqrt{3} \tan x + \sec(\sqrt{3}x)$$

$$(f) y = \frac{(x+2)^5 (e^x - 1)^2}{x^3 (x-1)^3} \Rightarrow \ln y = 5 \ln(x+2) + 2 \ln(e^x - 1) - 3 \ln x - 3 \ln(x-1)$$

$$\Rightarrow \frac{1}{y} \frac{dy}{dx} = \frac{5}{x+2} + \frac{2 \cdot e^x}{e^x - 1} - \frac{3}{x} - \frac{6}{x-1}$$

$$\Rightarrow \frac{dy}{dx} = \frac{(x+2)^5 (e^x - 1)^2}{x^3 (x-1)^3} \left(\frac{5}{x+2} + \frac{2e^x}{e^x - 1} - \frac{3}{x} - \frac{6}{x-1} \right)$$

$$3. y = \sin\left(\frac{\pi y}{x}\right) \Rightarrow \frac{dy}{dx} = \cos\left(\frac{\pi y}{x}\right) \cdot \pi \left(\frac{dy}{dx} \cdot \bar{x}^1 + y \cdot (-\bar{x}^{-2}) \right)$$

$$\Rightarrow \frac{dy}{dx} = 0 \quad \text{所求即 } y = 1 \quad *$$